Vegas/Graph.lean
@@ -11,3 +11,13 @@ import Vegas.Graph.MessagePolicyLaws
 import Vegas.Graph.MessageProgress
 import Vegas.Graph.MessageService
 import Vegas.Graph.MessageServiceLaw
+import Vegas.Graph.MessageServiceCursor
+import Vegas.Graph.MessageBindingLaw
+import Vegas.Graph.MessagePolicyCommands
+import Vegas.Graph.MessagePolicyHistory
+import Vegas.Graph.MessageServiceCompletion
+import Vegas.Graph.MessagePolicyFreshness
+import Vegas.Graph.MessageResolutionLaw
+import Vegas.Graph.MessageVerification
+import Vegas.Graph.MessageExpiryService
+import Vegas.Graph.MessageServiceTermination
